Remove location stores from op. semantics.

SmallStepSemantics.v
@@ -1,19 +1,18 @@
 Require Import Syntax.
 Require Import DbLib.DeBruijn.
 
-(* (sigma, e) -> (sigma', e') *)
-Inductive step : store -> term -> store -> term -> Prop :=
-  | StepAppAbs s e e' v t
+(* e ==> e' *)
+Inductive step : term -> term -> Prop :=
+  | StepAppAbs e e' v t
       (BetaPreVal : value v)
       (BetaPreSubst : subst v 0 e = e') :
-      step s (TApp (TAbs t e) v) s e'
-  | StepApp1 s s' e1 e1' e2
-      (App1Step : step s e1 s' e1') :
-      step s (TApp e1 e2) s' (TApp e1' e2)
-  | StepApp2 s s' v1 e2 e2'
+      step (TApp (TAbs t e) v) e'
+  | StepApp1 e1 e1' e2
+      (App1Step : step e1 e1') :
+      step (TApp e1 e2) (TApp e1' e2)
+  | StepApp2 v1 e2 e2'
       (App2Val : value v1)
-      (App2Step : step s e2 s' e2') :
-      step s (TApp v1 e2) s' (TApp v1 e2')
-.
+      (App2Step : step e2 e2') :
+      step (TApp v1 e2) (TApp v1 e2').
 
-Hint Constructors step.
+Hint Constructors step : l3.
